viper-total-heaps/TotalExtConsPreservation.thy
@@ -3,6 +3,11 @@ theory TotalExtConsPreservation
 begin
 
 
+lemma extcons_preserved_by_mh_change:
+  assumes "consistent_external ctxt \<phi>"
+  shows "consistent_external ctxt (upd_mh_total \<phi> mh')"
+  sorry
+
 lemma extcons_preserved_by_inhale_acc:
   assumes "consistent_external ctxt (get_total_full \<omega>)"
       and "\<omega>' \<in> inhale_perm_single StateCons \<omega> lh p_opt"
